:PROPERTIES:
:ID:       997b80e8-345d-46b4-b2dc-7e0856c11cdd
:mtime:    20220324095800
:ctime:    20220306174334
:END:
#+title: ?Proof of Vandermonde's identity using generating functions
#+filetags: :appendix:stub:

* Definition
Vandermonde's identity is the equality

\[
\binom{m+n}{r} = \sum\limits_{k=0}^r \binom{m}{k} \binom{n}{r-k}
\]

for non-negative integers \( r, m, n \).

* Generating functions
We may rewrite the identity in terms of generating functions as the equality

\[
\sum\limits_{r=0}^{m+n} \binom{m+n}{r} x^r = \sum\limits_{r=0}^{m+n} \sum\limits_{k=0}^{r}
\binom{m}{k} \binom{n}{r-k} x^r
\]

But now we notice that the right-hand side is nothing but a [[id:ddb31305-d703-45c7-8e5e-df361c9df07b][Convolution of generating functions]],
which we may rewrite as

\[
\sum\limits_{r=0}^{m+n} \sum\limits_{k=0}^r \binom{m}{k} \binom{n}{r-k} x^r = \left( \sum\limits_{i=0}^m
\binom{m}{i} x^i \right) \left( \sum\limits_{j=0}^n \binom{n}{j} x^j \right)
\]

Since the generating function of the binomial coefficients is \( (1+x)^p \), Vandermonde's identity
follows from

\[
(1 + x)^{m+n} = (1+x)^m (1+x)^n
\]
