:PROPERTIES:
:ID:       9eec1b8d-b4ed-4d77-a87d-afd9a84ae3bb
:mtime:    20220323210943
:ctime:    20220323205949
:END:
#+title: ?Renormalizing the exponential
#+filetags: :stub:

Consider the differential equation \( \dot{x}(t) = \epsilon x(t) \). The exact solution is \( x(t)
= x(0) e^{\epsilon t} \) and we would like to see if we can recover this behaviour through
renormalization.

Solving perturbatively, we find for \( x(t) = x_0(t) + x_1(t) \epsilon + O(\epsilon^2) \) the
solution

\begin{equation*}
\begin{align}
x_0(t) &= A \\
x_1(t) &= A (t-t_0)
\end{align}
\end{equation*}

so that \( x(t) = A \left( 1 + \epsilon (t-t_0) \right) + O(\epsilon^2) \).

We will denote this solution by \( x(t, t_0) \) to clarify the dependence on \( t_0 \).

Clearly, the naive solution breaks down when \( t-t_0 \) becomes large.

The renormalization technique tells us to make \( A \) dependent on \( t_0 \) and solve the RG
equations:

\begin{equation*}
\begin{align}
\frac{\partial x(t, t_0)}{\partial t_0} \big|_{t_0=t}
&= 0 \\
&= \left( \dot{A}(t_0) (1 + \epsilon (t-t_0)) + \epsilon A(t_0) \right) \big|_{t_0=t} \\
&= \dot{A}(t) + \epsilon A(t)
\end{align}
\end{equation*}

This has the solution \( A(t) = A(0) e^{\epsilon t} \). Now we plug this into our original solution
and set \( t_0 = t \). This leads to \( x(t) = A(t) = A(0) e^{\epsilon t} \) indeed recovering the
exact solution.
