:ctime:    20220320143640
:END:
#+title: Gumbel distribution
#+filetags: :stub:

With

\[
f(x) = \frac{1}{\beta} \exp \left( -\frac{x-\mu}{\beta} - e^{-\frac{x-\mu}{\beta}} \right)
\]

It is defined for \( x \in \mathbb{R} \). The [[denote:20220320T151714][Standard Gumbel distribution]] is obtained by setting
\( \mu = 0 \) and \( \beta = 1 \).

We have

\begin{equation*}
\begin{align}
\mathbb{E}[X]
&= \int\limits_{-\infty}^{\infty} \frac{x}{\beta} \exp \left( -\frac{x-\mu}{\beta} - e^{-\frac{x-\mu}{\beta}} \right) \, dx \\
&= \int\limits_{-\infty}^{\infty} \left( t + \frac{\mu}{\beta} \right) \exp \left( -t - e^{-t} \right) \, \beta dt \\
&= \int\limits_{-\infty}^{\infty} \left( \beta t + \mu \right) \exp \left( -t - e^{-t} \right) \, dt \\
&= \mu + \beta \int\limits_{-\infty}^{\infty} t  \exp \left( -t - e^{-t} \right) \, dt \\
\end{align}
\end{equation*}


\begin{equation*}
\begin{align}
\int\limits_{-\infty}^{\infty} t \exp \left( -t-e^{-t} \right) \, dt
&= \int\limits_0^{\infty} t \exp \left(-e^{-t} \right) \, de^{-t} \\
&= -\int\limits_0^{\infty} e^{-v} \log v \, dv \\
&= \gamma
\end{align}
\end{equation*}

# TODO: How to derive the third equality?
where \( \gamma \) is the [[denote:20220320T131858][Euler-Mascheroni constant]]. The third equality is a well-known equality.

This implies \( \mathbb{E}[X] = \mu + \beta \gamma \).

Moreover, [[denote:20220320T151935][?The difference of two Gumbel distributions is the logistic distribution]].
