:ctime:    20220227200208
:END:
#+title: The survival function is the exponential of the cumulative hazard function
#+filetags: :stub:

[[denote:20220227T162750][Hazard function]], [[denote:20220227T200014][Cumulative hazard function]]
# TODO: Express relation between survival function and hazard function

\begin{equation*}
\begin{align}
\mathbb{P}(t \leq T < t + h | T \geq t) &= \frac{\mathbb{P}(t \leq T < t + h)}{\mathbb{P}(T \geq t)} \\
&= \frac{\mathbb{P}(T \geq t) - \mathbb{P}(T \geq t + h)}{\mathbb{P}(T \ geq t)} \\
&= \frac{S(t) - S(t+h)}{S(t)}
\end{align}
\end{equation*}

Hence

\begin{equation*}
\begin{align}
\lambda(t) &= -\frac{1}{S(t)} \lim_{h \rightarrow 0^+} \frac{S(t+h) - S(t)}{h} \\
&= -\frac{\mathrm{d}}{\mathrm{d}t} \log S(t)
\end{align}
\end{equation*}

Hence

\[
S(t) = e^{-\int_0^t \lambda(u) \mathrm{d}u}
\]
