:ctime:    20220322115730
:END:
#+title: ?Renormalizing the damped harmonic oscillator
#+filetags: :appendix:stub:

Consider the damped harmonic oscillator equation:

\[
\ddot{x}(t) + \epsilon \dot{x}(t) + x(t) = 0
\]

Because this is a linear problem, we can find an exact solution of the form

\[
x(t) = A_0 e^{-\epsilon t / 2} \sin \left( t \sqrt{1 - \epsilon^2 / 4} + \phi_0} \right)
\]

We see two distinct effects due to the dampening:
- Decreasing amplitude (visible at \( O(\epsilon) \))
- Decreased frequency (visible at \( O(\epsilon^2) \))

Let us now calculate the perturbation result up to \( O(\epsilon^2) \) to show we can
recover these effects through renormalization, that would normally be invisible in standard
perturbation theory.

\begin{equation*}
\begin{align}
\ddot{x_0}(t) + x_0(t) &= 0 \\
\ddot{x_1}(t) + x_1(t) &= - \dot{x_0}(t) \\
\ddot{x_2}(t) + x_2(t) &= - \dot{x_1}(t)
\end{align}
\end{equation*}

Hence,

\begin{equation*}
\begin{align}
x_0(t) &= A(t_0) \sin(t + \phi(t_0)) \\
x_1(t) &= -\frac{A(t_0)}{2} (t-t_0) \sin(t + \phi(t_0)) \\
x_2(t) &= \frac{A(t_0)}{8} \left[ (t-t_0)^2 \sin(t + \phi(t_0)) - (t-t_0) \cos(t + \phi(t_0)) \right]
\end{align}
\end{equation*}

Now,

\begin{equation*}
\begin{align}
\frac{\partial x(t, t_0)}{\partial t_0}
&= \left( \dot{A} - \epsilon \frac{A}{2} \right) \sin(t + \phi) + \left( \dot{\phi} + \frac{\epsilon^2}{8} \right) A \cos(t + \phi) + (t-t_0) [...] + O(\epsilon^3) \\
&= 0
\end{align}
\end{equation*}

Since this has to be zero for any \( t \), we will find (after setting \( t_0 = t \))

\begin{equation*}
\begin{align}
\dot{A} &= \epsilon \frac{A}{2} \\
\dot{\phi} &= -\frac{\epsilon^2}{8}
\end{align}
\end{equation*}

These are the [[denote:20220322T105832][Renormalization group equations]].

We deliberately avoided calculating the terms that multiply the \( t-t_0 \) terms, because these
disappear anyway in when we set \( t_0 = t \).

The RG equations are solved by

\begin{equation*}
\begin{align}
A(t) &= A_0 e^{-\epsilon t / 2} \\
\phi(t) &= \phi_0 - \epsilon^2 t / 8
\end{align}
\end{equation*}

Plugging these results back in the original equation for \( x(t, t_0 = t) \), we find

\[
x(t) = A_0 e^{-\epsilon t / 2} \sin \left( t(1- \epsilon^2 / 8) + \phi_0 \right) + O(\epsilon^3)
\]

It should be noted that \( \sqrt{1 - \epsilon^2 / 4} = 1 - \epsilon^2 / 8 + O(\epsilon^4) \),
showing that we do indeed recover the expected frequency reduction as well.
