:ctime:    20220412204342
:END:
#+title: ?Derivation of the Euler-Lagrange equation
#+filetags: :appendix:stub:

We want to extremize

\[
S(y, \dot{y}, t) = \int\limits_{t_0}^{t_1} L(y, \dot{y}, t) \, dt
\]

Consider a small variation \( \tilde{y} = y + \epsilon \eta \). Then

\[
L(\tilde{y}, \dot{\tilde{y}}, t) = L(y, \dot{y}, t) + \epsilon \left( \eta \frac{\partial
L}{\partial y} + \dot{\eta} \frac{\partial L}{\partial \dot{y}} \right)
\]

so that

\[
S(\tilde{y}, \dot{\tilde{y}}, t) - S(y, \dot{y}, t) = \epsilon \int\limits_ {t_0}^{t_1} \left( \eta
\frac{\partial L}{\partial y} + \dot{\eta} \frac{\partial L}{\partial \dot{y}} \right) dt
\]

Applying integration by parts and constraining the endpoints such that \( \eta(t_0) = \eta(t_1)
= 0 \), we find

\[
\left[ \eta \frac{\partial L}{\partial \dot{y}} \right]_{t_0}^{t_1} = \int\limits_{t_0}^{t_1} \eta
\left( \frac{d}{dt} \frac{\partial L}{\partial \dot{y}} - \frac{\partial L}{\partial y} \right) \,
dt = 0
\]

Since this has to be true for any variation \( \eta \), we must find the [[denote:20220412T201834][Euler-Lagrange equation]]

\[
\frac{d}{dt} \frac{\partial L}{\partial \dot{y}} - \frac{\partial L}{\partial y} = 0
\]
