:ctime:    20220323092735
:END:
#+title: ?Rate function of the Bernoulli distribution
#+filetags: :appendix:stub:

The the Bernoulli distribution, it is known that the cumulant generating function is given by the
following expression:

\[
K(t) = \log \left( 1 + p(e^t - 1)) \right)
\]

This arises by replacing \( i t \) by \( t \) in the [[denote:20220323T093007][?Characteristic function of the Bernoulli
distribution]] and then taking the logarithm of the expression.

Now

\[
I(x) = \sup_{t>0} \left[ tx - K(t) \right]
\]

and the maximum of \( tx - K(t) \) is reached for \( K' (t) = x \) so that

\[
t = \log \frac{x(1-p)}{p(1-x)}
\]

Plugging this back into the definitions, we find

\begin{equation*}
\begin{align}
I(x)
&= x \log \frac{x(1-p)}{p(1-x)} - \log \left[ 1 + p \left( \frac{x(1-p)}{p(1-x)} - 1 \right) \right] \\
&= x \log \frac{x(1-p)}{p(1-x)} - \log \left[ \frac{1-p}{1-x} \right] \\
&= x \log x + (1-x) \log(1-x) - (1-x) \log(1-p) - x \log p \\
&= -S(x) - (1-x) \log(1-p) - x \log p \\
\end{align}
\end{equation*}

where \( S(x) \) is the [[denote:20220304T150924][?Entropy of the Bernoulli distribution]].
